feat: add user-defined fallback procedure for the `grind` tactic (#6512)
This PR introduces support for user-defined fallback code in the `grind`
tactic. The fallback code can be utilized to inspect the state of
failing `grind` subgoals and/or invoke user-defined automation. Users
can now write `grind on_failure <code>`, where `<code>` should have the
type `GoalM Unit`. See the modified tests in this PR for examples.

src/Lean/Elab/Tactic/Grind.lean
@@ -32,18 +32,36 @@ def elabGrindPattern : CommandElab := fun stx => do
         Grind.addEMatchTheorem declName xs.size patterns.toList
   | _ => throwUnsupportedSyntax
 
-def grind (mvarId : MVarId) (config : Grind.Config) (mainDeclName : Name) : MetaM Unit := do
-  let mvarIds ← Grind.main mvarId config mainDeclName
+def grind (mvarId : MVarId) (config : Grind.Config) (mainDeclName : Name) (fallback : Grind.Fallback) : MetaM Unit := do
+  let mvarIds ← Grind.main mvarId config mainDeclName fallback
   unless mvarIds.isEmpty do
     throwError "`grind` failed\n{goalsToMessageData mvarIds}"
 
+private def elabFallback (fallback? : Option Term) : TermElabM (Grind.GoalM Unit) := do
+  let some fallback := fallback? | return (pure ())
+  let type := mkApp (mkConst ``Grind.GoalM) (mkConst ``Unit)
+  let value ← withLCtx {} {} do Term.elabTermAndSynthesize fallback type
+  let auxDeclName ← if let .const declName _ := value then
+    pure declName
+  else
+    let auxDeclName ← Term.mkAuxName `_grind_fallback
+    let decl := Declaration.defnDecl {
+      name := auxDeclName
+      levelParams := []
+      type, value, hints := .opaque, safety := .safe
+    }
+    addAndCompile decl
+    pure auxDeclName
+  unsafe evalConst (Grind.GoalM Unit) auxDeclName
+
 @[builtin_tactic Lean.Parser.Tactic.grind] def evalApplyRfl : Tactic := fun stx => do
   match stx with
-  | `(tactic| grind $config:optConfig) =>
+  | `(tactic| grind $config:optConfig $[on_failure $fallback?]?) =>
+    let fallback ← elabFallback fallback?
     logWarningAt stx "The `grind` tactic is experimental and still under development. Avoid using it in production projects"
     let declName := (← Term.getDeclName?).getD `_grind
     let config ← elabGrindConfig config
-    withMainContext do liftMetaFinishingTactic (grind · config declName)
+    withMainContext do liftMetaFinishingTactic (grind · config declName fallback)
   | _ => throwUnsupportedSyntax
 
 end Lean.Elab.Tactic
