tests/lean/run/grind_congr.lean
@@ -4,53 +4,40 @@ def f (a : Nat) := a + a + a
 def g (a : Nat) := a + a
 
 -- Prints the equivalence class containing a `f` application
-open Lean Meta Elab Tactic Grind in
-elab "grind_test" : tactic => withMainContext do
-  let declName := (← Term.getDeclName?).getD `_main
-  Meta.Grind.preprocessAndProbe (← getMainGoal) declName do
-    let #[n, _] ← filterENodes fun e => return e.self.isAppOf ``f | unreachable!
-    let eqc ← getEqc n.self
-    logInfo eqc
+open Lean Meta Grind in
+def fallback : Fallback := do
+  let #[n, _] ← filterENodes fun e => return e.self.isAppOf ``f | unreachable!
+  let eqc ← getEqc n.self
+  logInfo eqc
+  (← get).mvarId.admit
 
 set_option grind.debug true
 set_option grind.debug.proofs true
 
 /--
 info: [d, f b, c, f a]
----
-warning: declaration uses 'sorry'
 -/
-#guard_msgs in
+#guard_msgs (info) in
 example (a b c d : Nat) : a = b → f a = c → f b = d → False := by
-  grind_test
-  sorry
+  grind on_failure fallback
 
 /--
 info: [d, f b, c, f a]
----
-warning: declaration uses 'sorry'
 -/
-#guard_msgs in
+#guard_msgs (info) in
 example (a b c d : Nat) : f a = c → f b = d → a = b → False := by
-  grind_test
-  sorry
+  grind on_failure fallback
 
 /--
 info: [d, f (g b), c, f (g a)]
----
-warning: declaration uses 'sorry'
 -/
-#guard_msgs in
+#guard_msgs (info) in
 example (a b c d e : Nat) : f (g a) = c → f (g b) = d → a = e → b = e → False := by
-  grind_test
-  sorry
+  grind on_failure fallback
 
 /--
 info: [d, f (g b), c, f v]
----
-warning: declaration uses 'sorry'
 -/
-#guard_msgs in
+#guard_msgs (info) in
 example (a b c d e v : Nat) : f v = c → f (g b) = d → a = e → b = e → v = g a → False := by
-  grind_test
-  sorry
+  grind on_failure fallback
