tests/lean/run/grind_norm_levels.lean
@@ -1,21 +1,17 @@
-import Lean
+import Lean.Meta.Tactic.Grind
 
 def g {α : Sort u} (a : α) := a
 
-open Lean Meta Elab Tactic Grind in
-elab "grind_test" : tactic => withMainContext do
-  let declName := (← Term.getDeclName?).getD `_main
-  Meta.Grind.preprocessAndProbe (← getMainGoal) declName do
-    let nodes ← filterENodes fun e => return e.self.isAppOf ``g
-    logInfo (nodes.toList.map (·.self))
+open Lean Meta Grind in
+def fallback : Fallback := do
+  let nodes ← filterENodes fun e => return e.self.isAppOf ``g
+  logInfo (nodes.toList.map (·.self))
+  (← get).mvarId.admit
 
 -- `grind` final state must contain only two `g`-applications
 /--
 info: [g (a, b), g (g (a, b))]
----
-warning: declaration uses 'sorry'
 -/
-#guard_msgs in
+#guard_msgs (info) in
 example {β : Type v} {α : Type u} (a c : α) (b d : β) : g.{max u v + 1} (a, b) = (c, d) → g (g.{max (u+1) (v+1)} (a, b)) = (c, d) → False := by
-  grind_test
-  sorry
+  grind on_failure fallback
