tests/lean/run/grind_propagate_connectives.lean
@@ -1,18 +1,16 @@
-import Lean
+import Lean.Meta.Tactic.Grind
 
--- Prints the equivalence class containing a `f` application
-open Lean Meta Elab Tactic Grind in
-elab "grind_test" : tactic => withMainContext do
-  let declName := (← Term.getDeclName?).getD `_main
-  Meta.Grind.preprocessAndProbe (← getMainGoal) declName do
-    let trueExprs := (← filterENodes fun e => return e.self.isFVar && (← isEqTrue e.self)).toList.map (·.self)
-    let falseExprs := (← filterENodes fun e => return e.self.isFVar && (← isEqFalse e.self)).toList.map (·.self)
-    logInfo m!"true:  {trueExprs}"
-    logInfo m!"false: {falseExprs}"
-    forEachEqc fun n => do
-      unless (← isProp n.self) || (← isType n.self) || n.size == 1 do
-        let eqc ← getEqc n.self
-        logInfo eqc
+open Lean Meta Grind in
+def fallback : Fallback := do
+  let trueExprs := (← filterENodes fun e => return e.self.isFVar && (← isEqTrue e.self)).toList.map (·.self)
+  let falseExprs := (← filterENodes fun e => return e.self.isFVar && (← isEqFalse e.self)).toList.map (·.self)
+  logInfo m!"true:  {trueExprs}"
+  logInfo m!"false: {falseExprs}"
+  forEachEqc fun n => do
+    unless (← isProp n.self) || (← isType n.self) || n.size == 1 do
+      let eqc ← getEqc n.self
+      logInfo eqc
+  (← get).mvarId.admit
 
 set_option grind.debug true
 set_option grind.debug.proofs true
@@ -21,73 +19,57 @@ set_option grind.debug.proofs true
 info: true:  [q, w]
 ---
 info: false: [p, r]
----
-warning: declaration uses 'sorry'
 -/
-#guard_msgs in
+#guard_msgs (info) in
 example : (p ∨ (q ∧ ¬r ∧ w)) → ¬p → False := by
-  grind_test
-  sorry
+  grind on_failure fallback
+
 
 /--
 info: true:  [r]
 ---
 info: false: [p, q]
----
-warning: declaration uses 'sorry'
 -/
-#guard_msgs in
+#guard_msgs (info) in
 example : (p ∨ q ∨ r) → (p ∨ ¬q) → ¬p → False := by
-  grind_test
-  sorry
+  grind on_failure fallback
+
 
 /--
 info: true:  [r]
 ---
 info: false: [p₁, q]
----
-warning: declaration uses 'sorry'
 -/
-#guard_msgs in
+#guard_msgs (info) in
 example : ((p₁ ∧ p₂) ∨ q ∨ r) → (p₁ ∨ ¬q) → p₁ = False → False := by
-  grind_test
-  sorry
+  grind on_failure fallback
 
 /--
 info: true:  [r]
 ---
 info: false: [p₂, q]
----
-warning: declaration uses 'sorry'
 -/
-#guard_msgs in
+#guard_msgs (info) in
 example : ((p₁ ∧ p₂) ∨ q ∨ r) → ((p₂ ∧ p₁) ∨ ¬q) → p₂ = False → False := by
-  grind_test
-  sorry
+  grind on_failure fallback
 
 /--
 info: true:  [q, r]
 ---
 info: false: [p]
----
-warning: declaration uses 'sorry'
 -/
-#guard_msgs in
+#guard_msgs (info) in
 example (p q r : Prop) : p ∨ (q ↔ r) → p = False → q → False := by
-  grind_test
-  sorry
+  grind on_failure fallback
 
 /--
 info: true:  [r]
 ---
 info: false: [p, s]
----
-warning: declaration uses 'sorry'
 -/
-#guard_msgs in
+#guard_msgs (info) in
 example (p q r : Prop) : p ∨ ¬(s ∨ (p ↔ r)) → p = False → False := by
-  grind_test
-  sorry
+  grind on_failure fallback
 
 /--
 info: true:  [p]
@@ -95,35 +77,29 @@ info: true:  [p]
 info: false: []
 ---
 info: [a, b]
----
-warning: declaration uses 'sorry'
 -/
-#guard_msgs in
+#guard_msgs (info) in
 example (p : Prop) (a : Vector Nat 5) (b : Vector Nat 6) : (p → HEq a b) → p → False := by
-  grind_test
-  sorry
-
+  grind on_failure fallback
 
 /--
 info: true:  [p, q]
 ---
 info: false: [r]
----
-warning: declaration uses 'sorry'
 -/
-#guard_msgs in
+#guard_msgs (info) in
 example (p q r : Prop) : p ∨ (q ↔ r) → q → ¬r → False := by
-  grind_test
-  sorry
+  grind on_failure fallback
 
 /--
+info: hello world
+---
 info: true:  [p, q]
 ---
 info: false: [r]
----
-warning: declaration uses 'sorry'
 -/
-#guard_msgs in
+#guard_msgs (info) in
 example (p q r : Prop) : p ∨ (q ↔ r) → ¬r → q → False := by
-  grind_test
-  sorry
+  grind on_failure do
+    Lean.logInfo "hello world"
+    fallback
