tests/lean/run/grind_ematch2.lean
@@ -41,3 +41,28 @@ example (as bs cs : Array α) (v₁ v₂ : α)
         (h₆ : j < as.size)
         : cs[j] = as[j] := by
   grind
+
+example (as bs cs ds : Array α) (v₁ v₂ v₃ : α)
+        (i₁ i₂ i₃ j : Nat)
+        (h₁ : i₁ < as.size)
+        (h₂ : as.set i₁ v₁ = bs)
+        (h₃ : i₂ < bs.size)
+        (h₃ : bs.set i₂ v₂ = cs)
+        (h₄ : i₃ < cs.size)
+        (h₅ : ds = cs.set i₃ v₃)
+        (h₆ : j ≠ i₁ ∧ j ≠ i₂ ∧ i₃ ≠ j)
+        (h₇ : j < ds.size)
+        (h₈ : j < as.size)
+        : ds[j] = as[j] := by
+  grind
+
+opaque f (a b : α) : α := a
+theorem fx : f x (f x x) = x := sorry
+grind_pattern fx => f x (f x x)
+
+/--
+info: [grind.ematch.instance] fx: f a (f a a) = a
+-/
+#guard_msgs (info) in
+example : a = b₁ → c = f b₁ b₂ → f a c ≠ a → a = b₂ → False := by
+  grind
